Notation; inputs/succ; general heap
Added notation commands to write the kind function out as g<<nid>>
to try to save some space and make definitions clearer.
Additionally added NoNode as empty which may be worth removing.

Changed the name of inp to inputs.
Changed the return of inputs and succ to sets as it is by
far the most common use case.

Changed DynamicHeap to a generic ('a, 'b) -> Value map.

IRGraph.thy
@@ -29,6 +29,9 @@ text_raw \<open>\Snip{graphdefnostamp}
 
 setup_lifting type_definition_IRGraph
 
+notation (latex)
+  NoNode ("\<epsilon>")
+
 text_raw \<open>\Snip{fake_lifted_helpers}\<close>
 fun ids_fake :: "(ID \<rightharpoonup> IRNode) \<Rightarrow> ID set" where
   "ids_fake g = {nid \<in> dom g . g nid \<noteq> (Some NoNode)}"
@@ -46,6 +49,9 @@ fun with_default :: "'c \<Rightarrow> ('b \<Rightarrow> 'c) \<Rightarrow> (('a \
 
 lift_definition kind :: "IRGraph \<Rightarrow> (ID \<Rightarrow> IRNode)"
   is "with_default NoNode fst" .
+
+notation (latex)
+  kind ("_\<llangle>_\<rrangle>")
 
 lift_definition stamp :: "IRGraph \<Rightarrow> ID \<Rightarrow> Stamp"
   is "with_default IllegalStamp snd" .
@@ -101,20 +107,20 @@ lemma [code]: "Rep_IRGraph (irgraph m) = map_of (no_node m)"
 
 text_raw \<open>\Snip{helpers}%\<close>
 (* Get the inputs list of a given node ID. *)
-fun inp :: "IRGraph \<Rightarrow> ID \<Rightarrow> ID list" where
-  "inp g nid = (inputs_of (kind g nid))"
+fun inputs :: "IRGraph \<Rightarrow> ID \<Rightarrow> ID set" where
+  "inputs g nid = set (inputs_of (kind g nid))"
 (* Get the successor list of a given node ID. *)
-fun succ :: "IRGraph \<Rightarrow> ID \<Rightarrow> ID list" where
-  "succ g nid = (successors_of (kind g nid))"
+fun succ :: "IRGraph \<Rightarrow> ID \<Rightarrow> ID set" where
+  "succ g nid = set (successors_of (kind g nid))"
 (* Gives a relation between node IDs - between a node and its input nodes. *)
 fun input_edges :: "IRGraph \<Rightarrow> ID rel" where
-  "input_edges g = (\<Union> i \<in> ids g. {(i,j)|j. j \<in> fset(fset_of_list (inp g i))})"
+  "input_edges g = (\<Union> i \<in> ids g. {(i,j)|j. j \<in> (inputs g i)})"
 (* Find all the nodes in the graph that have nid as an input. *)
 fun usages :: "IRGraph \<Rightarrow> ID \<Rightarrow> ID set" where
   "usages g nid = {j. j \<in> ids g \<and> (j,nid) \<in> input_edges g}"
 
 fun successor_edges :: "IRGraph \<Rightarrow> ID rel" where
-  "successor_edges g = (\<Union> i \<in> ids g. {(i,j)|j . j \<in> fset(fset_of_list (succ  g i))})"
+  "successor_edges g = (\<Union> i \<in> ids g. {(i,j)|j . j \<in> (succ  g i)})"
 
 fun predecessors :: "IRGraph \<Rightarrow> ID \<Rightarrow> ID set" where
   "predecessors g nid = {j. j \<in> ids g \<and> (j,nid) \<in> successor_edges g}"
@@ -139,8 +145,8 @@ text_raw \<open>\Snip{wff_closed}%\<close>
 definition wff_closed where
   "wff_closed g = 
     (\<forall> n \<in> ids g .
-      set (inp g n) \<subseteq> ids g \<and>
-      set (succ g n) \<subseteq> ids g \<and>
+      inputs g n \<subseteq> ids g \<and>
+      succ g n \<subseteq> ids g \<and>
       kind g n \<noteq> NoNode)"
 text_raw \<open>\EndSnip\<close>
 
